Transformation.thy
@@ -2,10 +2,10 @@ theory Transformation
   imports Big Small
 begin
 
-fun ticksHelper :: "'a Big.state \<Rightarrow> 'a Small.state \<Rightarrow> 'a Big.state * 'a Small.state" where
-  "ticksHelper (Reverse currentB big auxB 0) (Reverse1 currentS _ auxS) =
+fun ticksHelper :: "('a Big.state * 'a Small.state) \<Rightarrow> 'a Big.state * 'a Small.state" where
+  "ticksHelper (Reverse currentB big auxB 0, Reverse1 currentS _ auxS) =
     (Big.Common (normalize (Copy currentB auxB [] 0)), Reverse2 currentS auxS big [] 0)"
-| "ticksHelper left right = (Big.tick left, Small.tick right)"
+| "ticksHelper (left, right) = (Big.tick left, Small.tick right)"
 
 datatype 'a transformation =
    Left "'a Small.state" "'a Big.state"
@@ -20,8 +20,8 @@ fun toListRight :: "'a transformation \<Rightarrow> 'a list" where
 | "toListRight (Right big small) = Small.toList small @ (rev (Big.toList big))"
 
 fun ticks :: "'a transformation \<Rightarrow> 'a transformation" where
-  "ticks (Left small big) = (case ticksHelper big small of (big, small) \<Rightarrow> Left small big)"
-| "ticks (Right big small) = (case ticksHelper big small of (big, small) \<Rightarrow> Right big small)"  
+  "ticks (Left small big) = (case ticksHelper (big, small) of (big, small) \<Rightarrow> Left small big)"
+| "ticks (Right big small) = (case ticksHelper (big, small) of (big, small) \<Rightarrow> Right big small)"  
 
 fun fourTicks where
   "fourTicks transformation = (ticks (ticks (ticks (ticks transformation))))"
