Common_Proof.thy
@@ -1,9 +1,15 @@
 theory Common_Proof
-  imports Common
+  imports Common Current_Proof
 begin
 
 lemma tick: "toList (tick common) = toList common"
   apply(induction common)
   by(auto split: current.splits)
 
+lemma push:  "toList (push x common) = x # toList common"
+  apply(induction common arbitrary: x)
+  apply(auto simp: put)
+  (* TODO: *)
+  by (metis Common.push.simps(1) Common.toList.simps(1) idle.exhaust put)
+  
 end
