Current_Proof.thy
@@ -1,0 +1,9 @@
+theory Current_Proof
+  imports Current
+begin
+
+lemma put: "toList (put x current) = x # Current.toList current"
+  apply(induction x current rule: put.induct)
+  by auto
+
+end
