Transformation_Proof.thy
@@ -1,44 +1,36 @@
 theory Transformation_Proof
-  imports Transformation Small_Proof Big_Proof Stack_Proof
+  imports Transformation Small_Proof Big_Proof Stack_Proof Current_Proof
 begin
 
 lemmas tick = Small_Proof.tick Big_Proof.tick Common_Proof.tick
 
+lemma ticks_help: "ticksHelper (big, small) = (newBig, newSmall) \<Longrightarrow> Big.toList big = Big.toList newBig"
+  apply(induction "(big, small)" rule: ticksHelper.induct)
+  by(auto simp: tick split: current.splits if_splits)
+
+lemma ticks_help2: "ticksHelper (big, small) = (newBig, newSmall) \<Longrightarrow> Small.toList small = Small.toList newSmall"
+  apply(induction "(big, small)" rule: ticksHelper.induct)
+  by(auto simp: tick split: current.splits if_splits)
+
 lemma ticks: "toListLeft (ticks transformation) = toListLeft transformation"
-proof(induction transformation rule: toListLeft.induct)
-  case (1 small big)
-  
-  have "\<And>right left. 
-        ticksHelper big small = (right, left) \<Longrightarrow>
-        Small.toList small @ rev (Big.toList big) = Small.toList left @ rev (Big.toList right)"
-    apply(induction big small rule: ticksHelper.induct)
-    by(auto simp: tick split: current.splits)
+  apply(induction transformation rule: toListLeft.induct)
+  by(auto simp: ticks_help ticks_help2 split: prod.splits)
 
-  then show ?case
-    by (auto split: prod.splits)
-next
-  case (2 big small)
 
-  have "\<And>left right. 
-        ticksHelper big small = (left, right) \<Longrightarrow>
-        Big.toList big @ rev (Small.toList small) = Big.toList left @ rev (Small.toList right)"
-    apply(induction big small rule: ticksHelper.induct)
-    by(auto simp: tick split: current.splits)
+lemmas all_ticks = tick ticks
 
-  then show ?case
-    by(auto split: prod.splits)
-qed
+lemmas state_splits = idle.splits Common.state.splits Small.state.splits Big.state.splits 
 
-(* TODO: *)
+
 lemma ticks_helper: "\<lbrakk>
   ticksHelper
-         (Reverse (Current [] 0 (Stack.push x leftValues) (Stack.size leftValues - Stack.size rightValues)) (Stack.push x leftValues) [] (Stack.size leftValues - Stack.size rightValues))
-         (Reverse1 (Current [] 0 rightValues (Suc (2 * Stack.size rightValues))) rightValues []) = (left, right)
+         (Reverse (Current [] 0 (Stack.push x leftValues) (Stack.size leftValues - Stack.size rightValues)) (Stack.push x leftValues) [] (Stack.size leftValues - Stack.size rightValues),
+         Reverse1 (Current [] 0 rightValues (Suc (2 * Stack.size rightValues))) rightValues []) = (left, right)
     \<rbrakk>
        \<Longrightarrow> Big.toList left @ rev (Small.toList right) = x # Stack.toList leftValues @ rev (Stack.toList rightValues)"
 proof(induction  
-         "Reverse (Current [] 0 (Stack.push x leftValues) (Stack.size leftValues - Stack.size rightValues)) (Stack.push x leftValues) [] (Stack.size leftValues - Stack.size rightValues)"
-         "Reverse1 (Current [] 0 rightValues (Suc (2 * Stack.size rightValues))) rightValues []"
+         "(Reverse (Current [] 0 (Stack.push x leftValues) (Stack.size leftValues - Stack.size rightValues)) (Stack.push x leftValues) [] (Stack.size leftValues - Stack.size rightValues)
+         , Reverse1 (Current [] 0 rightValues (Suc (2 * Stack.size rightValues))) rightValues [])"
         rule: ticksHelper.induct
         )
   case 1
@@ -54,8 +46,134 @@ next
      by(auto simp: push split: if_splits)
  qed
 
-lemmas all_ticks = tick ticks ticks_helper
 
-lemmas state_splits = idle.splits Common.state.splits Small.state.splits Big.state.splits 
+
+lemma test_2_1: "put x current = Current x1 x2 x3 x4 
+        \<Longrightarrow> x1 @ Stack.toList x3 = x # Current.toList current"
+  apply(induction x current rule: put.induct)
+  by auto
+
+lemma small_push: "x # Small.toList small = Small.toList (Small.push x small) "
+  apply(induction x small rule: Small.push.induct)
+  by(auto simp: Common_Proof.push put)
+
+lemma test_2: "ticksHelper (big, Small.push x small) = (big', small')
+           \<Longrightarrow> Small.toList small' = x # Small.toList small"
+  by(auto simp: small_push ticks_help2)
+
+
+lemma test: " \<lbrakk>
+    ticksHelper (x1b, x2b) = (x1c, small'); 
+    ticksHelper (x1a, x2a) = (x1b, x2b); 
+    ticksHelper (x1, x2) = (x1a, x2a);
+    ticksHelper (right, Small.push x left) = (x1, x2)\<rbrakk>
+       \<Longrightarrow> Small.toList small' = x # Small.toList left"
+  by (metis ticks_help2 test_2)
+
+lemma something_1_1: "\<lbrakk>
+      ticksHelper (right, Small.push x left) = (Big.state.Common (state.Idle x21a (idle.Idle x1e x2f)), Small.state.Common (state.Idle x21 (idle.Idle x1d x2d)))
+    \<rbrakk> \<Longrightarrow> Stack.toList x1d  = x # Small.toList left"
+    apply(induction "(right, Small.push x left)" rule: ticksHelper.induct;
+        induction x left rule: Small.push.induct;
+        induction x1d rule: Stack.toList.induct;
+        induction x1e rule: Stack.toList.induct;
+        induction right;
+        induction x21a arbitrary:  x2d x2f rule: Current.toList.induct;
+        induction x21 rule: Current.toList.induct)
+                      apply(auto simp: tick split: if_splits current.splits)
+  
+  sorry
+
+lemma something_1: "\<lbrakk>
+      ticksHelper (right, Small.push x left) = (Big.state.Common (state.Idle x21a (idle.Idle x1e x2f)), Small.state.Common (state.Idle x21 (idle.Idle x1d x2d)))
+    \<rbrakk> \<Longrightarrow> Stack.toList x1d @ rev (Stack.toList x1e) = x # Small.toList left @ rev (Current.toList x21a)"
+  apply(auto simp: something_1_1)
+  apply(induction x1e rule: Stack.toList.induct;
+        induction x21a rule: Current.toList.induct;
+        induction x left rule: Small.push.induct;
+        induction right
+        )
+       apply(auto split: if_splits current.splits)    
+    apply(induction x21 arbitrary: x2f x2d; induction x1d  rule: Stack.toList.induct)
+  
+  sorry
+
+lemma something: " \<lbrakk>
+        ticksHelper (x1b, x2b) = (Big.state.Common (state.Idle x21a (idle.Idle x1e x2f)), Small.state.Common (state.Idle x21 (idle.Idle x1d x2d)));
+        ticksHelper (x1a, x2a) = (x1b, x2b); 
+        ticksHelper (x1, x2) = (x1a, x2a); 
+      ticksHelper (right, Small.push x left) = (x1, x2)
+    \<rbrakk> \<Longrightarrow> Stack.toList x1d @ rev (Stack.toList x1e) = x # Small.toList left @ rev (Current.toList x21a)"
+  apply(induction "(right, Small.push x left)" rule: ticksHelper.induct;
+        induction x1d rule: Stack.toList.induct;
+        induction x1e rule: Stack.toList.induct;
+        induction left arbitrary: x rule: Small.toList.induct)
+  (*apply(auto split: current.splits if_splits)*)
+  sorry
+
+(*
+lemma test1_1_1: "put x r1 = Current r1' r2' r3' r4' \<Longrightarrow> r1' @ Stack.toList r3' = x # Current.toList r1"
+  apply(induction r1 rule: Current.toList.induct)
+  by auto
+
+lemma test1_1: "
+       ticksHelper (Reverse l1 l2 l3 l4) (Reverse1 (put x r1) r2 r3) =
+       (Reverse l1' l2' l3' l4', Reverse1 (Current r1' r2' r3' r4') small auxS) \<Longrightarrow>
+       r1' @ Stack.toList r3' @ rev (Current.toList l1') = x # Current.toList r1 @ rev (Current.toList l1)"
+  apply(induction "Reverse l1 l2 l3 l4" "Reverse1 (put x r1) r2 r3" rule: ticksHelper.induct)
+  by(auto simp: test1_1_1 split: if_splits)
+
+lemma test1_2: "\<lbrakk>
+    put x current = Current extra added old remained
+  \<rbrakk> \<Longrightarrow> extra @ Stack.toList old @ rev (Common.toList (Common.tick common)) = x # Current.toList current @ rev (Common.toList common)"
+  apply(induction current rule: Current.toList.induct)
+  by(auto simp: tick)
+
+lemma test1_3: "
+      ticksHelper (Reverse x1 x2aa x3 x4) (Reverse1 (put xa x1aa) x2 x3aa) = 
+      (Big.state.Common x, Reverse1 (Current x1a x2a x3a x4a) small auxS)
+       \<Longrightarrow>
+      x1a @ Stack.toList x3a @ rev (Common.toList x) = xa # Current.toList x1aa @ rev (Current.toList x1)"
+  apply(induction "Reverse x1 x2aa x3 x4" "Reverse1 (put xa x1aa) x2 x3aa" rule: ticksHelper.induct)
+  by auto
+
+lemma test1: "\<lbrakk>
+  ticksHelper right (Small.push x left) = (big, Reverse1 current small auxS)
+  \<rbrakk> \<Longrightarrow> Current.toList current @ rev (Big.toList big) = x # Small.toList left @ rev (Big.toList right)"
+  apply(induction left; induction right; induction big; induction current arbitrary: x small auxS)
+  by(auto simp: test1_1 test1_2 test1_3 split: if_splits)
+
+lemma test2_1: "\<lbrakk>
+  Reverse1 currentS uu auxS = Small.push x left;
+  Small.tick right = Reverse1 x11 x12 x13;
+  ticksHelper (Reverse currentB big auxB 0) (Small.push x left) = (Reverse v va vb (Suc vd), right)
+  \<rbrakk> \<Longrightarrow> Current.toList x11 @ rev (Current.toList v) = x # Small.toList left @ rev (Current.toList currentB)"
+  apply(induction "Reverse currentB big auxB 0" "Small.push x left" rule: ticksHelper.induct;
+        induction x11 rule: Current.toList.induct;
+        induction currentB rule: Current.toList.induct;
+        induction left rule: Small.toList.induct;
+        induction v arbitrary: x rule: Current.toList.induct)
+  by auto
+
+lemma test2: "\<lbrakk>
+  ticksHelper x1 x2 = (x1c, Reverse1 x11 x12 x13); 
+  ticksHelper right (Small.push x left) = (x1, x2)
+  \<rbrakk> \<Longrightarrow> Current.toList x11 @ rev (Big.toList x1c) = x # Small.toList left @ rev (Big.toList right)"
+  apply(induction right "Small.push x left" rule: ticksHelper.induct;
+        induction x1 x2 arbitrary: x left x11 x12 x13 x1c  rule: ticksHelper.induct)
+   apply(auto simp: test2_1 split: if_splits)
+  sorry
+
+lemma test: "\<lbrakk>
+  ticksHelper x1b x2b = (x1c, Reverse1 x11 x12 x13); 
+  ticksHelper x1a x2a = (x1b, x2b); 
+  ticksHelper x1 x2 = (x1a, x2a);
+  ticksHelper right (Small.push x left) = (x1, x2)
+  \<rbrakk> \<Longrightarrow> Current.toList x11 @ rev (Big.toList x1c) = x # Small.toList left @ rev (Big.toList right)"
+  apply(auto simp: ticks_help ticks_help2)
+(*apply(induction right "Small.push x left" rule: ticksHelper.induct;
+        induction x1 x2 rule: ticksHelper.induct;
+        induction x1a x2a rule: ticksHelper.induct)*)
+  sorry*)
 
 end
